basic hash from two independent urns (wip)

theories/elton/examples/basic_hash.v
@@ -1,5 +1,6 @@
 From iris.base_logic.lib Require Import token.
-From clutch.elton Require Import elton hash. 
+From clutch.elton Require Import elton hash
+  (* examples.finset_bijection examples.gset_bij_lift *).
 Set Default Proof Using "Type*".
 
 (** https://github.com/proof-ladders/protocol-ladder/blob/main/Notes/main.pdf
@@ -67,9 +68,1097 @@ Section prog.
 
       let: "g" := "A" ("n1", "h1") ("n2", "h2") "hashf'"  in
       "g" = "b".
-  
-  (* Context `{eltonGS Σ}. *)
 
+  Definition prog_two_urns : expr :=
+    λ: "A",
+      let: "hashf" := init_hash val_size #() in
+      let: "b" := rand #1 in
+      let: "T1" := rand #(tag_range) in
+      let: "T2" := "b" * "T1" + (#1-"b") * rand #(tag_range) in
+      let: "n1" := rand #nonce_range in
+      (* Pay error for n2 to avoid colliding with n1*)
+      let: "n2" := rand #nonce_range in
+      let: "h1" := "hashf" ("n1"*#(tag_range+1) +"T1") in
+      let: "h2" := "hashf" ("n2"*#(tag_range+1) +"T2") in
+
+      let: "i" := ref #tries in
+      let: "hashf'" :=
+        (λ: "x", if: ! "i" = #0
+                 then NONE
+                 else "i" <- ! "i" - #1;; SOME ("hashf" "x") ) in
+
+      let: "g" := "A" ("n1", "h1") ("n2", "h2") "hashf'" in
+      "g" = "b".
+
+  Definition prog_two_urns_delayed : expr :=
+    λ: "A",
+      let: "hashf" := init_hash val_size #() in
+      let: "b" := drand #1 in
+      let: "T1" := drand #(tag_range) in
+      let: "T2" := "b" * "T1" + (#1-"b") * drand #(tag_range) in
+      let: "n1" := rand #nonce_range in
+      (* Pay error for n2 to avoid colliding with n1*)
+      let: "n2" := rand #nonce_range in
+      let: "h1" := "hashf" ("n1"*#(tag_range+1) +"T1") in
+      let: "h2" := "hashf" ("n2"*#(tag_range+1) +"T2") in
+
+      let: "i" := ref #tries in
+      let: "hashf'" :=
+        (λ: "x", if: ! "i" = #0
+                 then NONE
+                 else "i" <- ! "i" - #1;; SOME ("hashf" "x") ) in
+
+      let: "g" := "A" ("n1", "h1") ("n2", "h2") "hashf'" in
+      "g" = "b".
+
+
+  (* Definition zedprod_inv (N : Z) (Npos : (0 < N)%Z) (s : gset (fin ((Z.to_nat N) * (Z.to_nat N))))
+       : prodset (fin (Z.to_nat N)) (fin (Z.to_nat N))
+       := FS_bij ((gset_bij_lift (finset_bij_fun N Npos)) s).
+
+     Definition zedprod (N : Z) (Npos : (0 < N)%Z) (s1_s2 : prodset (fin (Z.to_nat N)) (fin (Z.to_nat N)))
+       : gset (fin ((Z.to_nat N) * (Z.to_nat N)))
+       := (gset_bij_lift (f_inv $ finset_bij_fun N Npos)) (FS_bij_inv s1_s2).
+
+     #[local] Instance zedprod_inv_inj {N : Z} {h : (0 < N)%Z} : Inj eq eq (zedprod_inv N h).
+     unfold zedprod_inv.
+     eapply (compose_inj eq eq eq _ FS_bij) ;
+       try apply _. apply FS_bij_TC.
+     Defined.
+
+     #[local] Instance zedprod_inv_surj {N : Z} {h : (0 < N)%Z} : Surj eq (zedprod_inv N h).
+     unfold zedprod_inv.
+     eapply (compose_surj eq _ FS_bij) ;
+       try apply _. apply FS_bij_TC.
+     Defined.
+
+
+     #[local] Instance zedprod_bij {N : Z} {h : (0 < N)%Z} : Inj eq eq (zedprod N h).
+     unfold zedprod.
+     eapply compose_inj.
+     intros ?? heq.
+
+     apply _.
+     #[local] Instance zedprod_bij {N : Z} {h : 0 < N} : Bij (zedprod N h).
+     rewrite /zedprod. split ; apply _. *)
+
+
+  Lemma basic_hash_game_two_urns A:
+    ∅ ⊢ₜ A : ((TInt* TInt) → (TInt* TInt) → (TInt → (TUnit+TInt))  → TInt) ->
+             pgl (lim_exec ((prog_two_urns A), {|heap:=∅; urns:= ∅|})) (λ v, v=#false)
+               (1/2 + 1/(nonce_range +1 )%nat + (2*(tries)%nat)/(tag_range+1)%nat).
+  Proof.
+    intros Htyped.
+    destruct (decide (2*(tries)<tag_range+1)) as [initial_ineq|]; last first.
+    {
+      apply pgl_1.
+      apply Rle_plus_r; last first.
+      - apply Rle_plus_r; last lra. apply Rdiv_INR_ge_0.
+      - apply Rcomplements.Rle_div_r; first (apply Rlt_gt; apply lt_0_INR; lia).
+        rewrite Rmult_1_l.
+        replace 2%R with (INR 2) by done.
+        rewrite -mult_INR.
+        apply le_INR.
+        lia.
+    }
+    eapply (elton_adequacy_remove_drand (#[eltonΣ; tokenΣ]) (prog_two_urns_delayed A)).
+    { simpl; by erewrite typed_remove_drand_expr. }
+    { apply Rplus_le_le_0_compat; last real_solver.
+      apply Rplus_le_le_0_compat; first lra. apply Rdiv_INR_ge_0. }
+    rewrite /prog_two_urns_delayed.
+    iIntros (? Φ).
+    iModIntro.
+    iIntros "Herr HΦ".
+
+    iPoseProof (typed_safe _ [] _ Htyped) as "H".
+    wp_bind (A).
+    iApply (pgl_wp_wand); first done.
+    iIntros (?) "#Hinterp".
+    simpl.
+    wp_pures.
+
+
+    wp_apply (wp_init_hash); first done.
+    iIntros (f) ">Hf".
+    wp_pures.
+
+    wp_apply (wp_drand_thunk _ _ _ _ _ (True)).
+    { rewrite rupd_unseal/rupd_def.
+      iIntros (?) "$".
+      iPureIntro.
+      intros.
+      simpl.
+      eexists _; split; first done.
+      f_equal.
+      f_equal.
+      instantiate (1:=1).
+      lia. }
+      iIntros (b) "[_ Hb]".
+      rewrite Nat2Z.id.
+      wp_pures.
+
+    wp_apply (wp_drand_thunk _ _ _ _ _ (True)).
+    { rewrite rupd_unseal/rupd_def.
+      iIntros (?) "$".
+      iPureIntro.
+      intros.
+      simpl.
+      eexists _; split; first done.
+      f_equal.
+      f_equal.
+      instantiate (1:=(tag_range)).
+      lia. }
+      iIntros (l) "[_ Hl]".
+      rewrite Nat2Z.id.
+      wp_pures.
+
+    wp_apply (wp_drand_thunk _ _ _ _ _ (True)).
+    { rewrite rupd_unseal/rupd_def.
+      iIntros (?) "$".
+      iPureIntro.
+      intros.
+      simpl.
+      eexists _; split; first done.
+      f_equal.
+      f_equal.
+      instantiate (1:=(tag_range)).
+      lia. }
+      iIntros (l') "[_ Hl']".
+      rewrite Nat2Z.id.
+      wp_pures.
+
+      wp_apply wp_rand; first done.
+      iIntros (n1) "_".
+      wp_pures.
+
+      iDestruct (ec_split with "[$]") as "[Herr1 Herr2]"; [|real_solver|].
+      { apply Rplus_le_le_0_compat; real_solver. }
+
+
+      iDestruct (ec_split with "[$Herr1]") as "[Herr1 Herr1']"; [real_solver..|].
+
+      wp_apply (wp_couple_rand_adv_comp' _ _ _ _ (λ x, if bool_decide (x = n1) then nnreal_one else nnreal_zero)with "[$Herr1']").
+      { intros. case_bool_decide; simpl; lra. }
+      { rewrite SeriesC_scal_l. rewrite SeriesC_singleton.
+        rewrite Rmult_1_r.
+        rewrite S_INR. by rewrite plus_INR.
+      }
+      iIntros (n2) "Herr1'".
+      case_bool_decide as nonce_neq; first (by iDestruct (ec_contradict with "[$Herr1']") as "[]").
+      wp_pures.
+      iClear "Herr1'".
+
+      iMod (ec_zero) as "Hzero".
+      wp_apply (wp_insert_new _ _ _ _ _ _ (λ _, 0)%R True with "[$Hf $Hzero]").
+      { done. }
+      { by intros. }
+      { right. apply SeriesC_0. intros. lra. }
+      { iModIntro. rewrite dom_empty_L. by rewrite big_sepS_empty. }
+      iIntros (h1) "(Hf&_)".
+      wp_pures.
+
+      iMod (ec_zero) as "Hzero".
+      wp_apply (wp_insert_new _ _ _ _ _ _ (λ _, 0)%R ((l↪ _) ∗ (l'↪ _) ∗ (b↪ _)) with "[$Hf $Hzero $Hl $Hl' $Hb]").
+      { done. }
+      { by intros. }
+      { right. apply SeriesC_0. intros. lra. }
+      { iModIntro.
+        rewrite insert_empty.
+        rewrite dom_singleton_L.
+        iApply big_sepS_intro.
+        iModIntro.
+        iIntros (?) "%Hlookup'".
+        iIntros "[Hl [Hl' Hb]]".
+
+        rewrite rupd_unseal/rupd_def.
+        iIntros  (?) "[? Hu]". iSplit; last iFrame.
+        iDestruct (ghost_map_lookup with "Hu [$Hb]") as "%Hlookup_b".
+        iDestruct (ghost_map_lookup with "Hu [$Hl]") as "%Hlookup_l".
+        iDestruct (ghost_map_lookup with "Hu [$Hl']") as "%Hlookup_l'".
+        iPureIntro.
+        intros.
+        exists false. split => //.
+        eapply urns_f_distr_lookup in Hlookup_l ; last done.
+        2:{ admit. }
+        eapply urns_f_distr_lookup in Hlookup_l' ; last done.
+        2:{ admit. }
+        eapply urns_f_distr_lookup in Hlookup_b ; last done.
+        2:{ admit. }
+        destruct Hlookup_l as (?&Hsome_l&Hin).
+        destruct Hlookup_l' as (?&Hsome_l'&Hin_l').
+        destruct Hlookup_b as (?&Hsome_b&Hin').
+        simpl.
+        rewrite Hsome_l Hsome_l' Hsome_b. simpl.
+        set_unfold in Hlookup'. simplify_eq.
+        simpl. rewrite Hsome_l. simpl. f_equal.
+        case_bool_decide as hh ; try done. exfalso.
+        clear -hh nonce_neq Hin Hin' Hin_l'.
+        simpl in Hin'.
+        set_unfold in Hin'.
+        set_unfold in Hin.
+        set_unfold in Hin_l'.
+        destruct Hin as [? [? []]]. simplify_eq.
+        destruct Hin_l' as [? [? []]]. simplify_eq.
+
+        opose proof (Zdiv_mod_unique (tag_range+1) n1 n2
+                       (x)
+                       (x2 * x + (1 - x2) * x0)
+                       _ _) as h.
+
+        - apply Zabs_ind ; intros ; try lia.
+        - apply Zabs_ind ; intros ; try lia.
+        - apply nonce_neq.
+          unshelve epose proof (h _) as [] ; last by simplify_eq.
+          lia.
+      }
+      iIntros (h2) "(Hf&(Hl&Hl'&Hb)&_)".
+      wp_pures.
+
+      wp_alloc lt as "Hr".
+      wp_pures.
+  (*
+    Let k1 = l/S tag_range and k2 = l%S tag_range
+     Here h1 is storing h (n1 || k1)
+     Here h2 is storing either h (n2 || k1) or (n2 || l%k2)
+
+     Let s1 be the range of values k1 can be, similarly be s2.
+     This means initially s1 and s2 = {0, ... , tag_range}
+     Initially the urn l is storing s1 ** s2,
+     where (x ** y) is a set of all elements (a*S tag_range + b) for all a in x, b in y
+
+     Now each time the adversary queries the hash, say with input i,
+     let i' = i%(S tag_range), we pay errors to ensure i' is not stored in s1 or s2
+     This way, i is never (n1||k1) or (n2||k2)
+
+     The adversary gets "tries" attempt, and a 1/2 chance to get the b correct
+
+     Hence the error is 2*(tries)/(S tag_range) + 1/2
+   *)
+      (* set (ff (x y : Z) := (x * tag_range + y)%Z).
+         set (f' := (λ (xy : Z * Z), ff xy.1 xy.2)).
+         set (g (s1 s2 : gset Z) := (cprod s1 s2 : gset (Z * Z))).
+         set (h := set_map (A := (Z*Z)) (B := Z)
+                     (C := gset (Z*Z))
+                     (D := gset Z)
+                      f').
+         set (setprod (s1 s2 : gset Z) := h (g s1 s2)).
+         set (n1_b_n2_T2 := ((n2 * (tag_range + 1))%Z +ᵥ
+                  ((LitLbl b *ᵥ QuotOp' (LitLbl l) (tag_range + 1)%Z) +ᵥ
+                   ((1%Z -ᵥ LitLbl b) *ᵥ RemOp' (LitLbl l) (tag_range + 1)%Z)))%V).
+         set (n1_T1 := ((n1 * (tag_range + 1))%Z +ᵥ
+                     QuotOp' (LitLbl l) (tag_range + 1)%Z)%V). *)
+
+      iMod (token_alloc) as (γ) "Htoken".
+
+      set (n1_b_n2_T2 := ((n2 * (tag_range + 1))%Z +ᵥ
+               ((LitLbl b *ᵥ LitLbl l) +ᵥ ((1%Z -ᵥ LitLbl b) *ᵥ LitLbl l')))%V).
+      set (n1_T1 := ((n1 * (tag_range + 1))%Z +ᵥ LitLbl l)%V).
+      set (inv :=
+  ( ∃ (tries':nat) (m:gmap Z nat) (x y : fin (S val_size)),
+             hashfun val_size f (<[n1_b_n2_T2:=fin_to_nat x]> (<[n1_T1:=fin_to_nat y]> (kmap (λ x, LitInt (x)) m)))∗
+             lt ↦ #tries' ∗ (⌜(tries'<=tries)%nat ⌝) ∗
+             ∃ (s : gset Z),
+               ⌜∀ x : Z, x ∈ s -> (n1 * (tag_range + 1) + x ∉ ((dom m) : gset _))%Z⌝ ∗
+               ⌜∀ x : Z, x ∈ s -> (n2 * (tag_range + 1) + x ∉ ((dom m) : gset _))%Z⌝ ∗
+
+               ⌜∀ x : Z, x ∈ s -> 0 <= x <= tag_range⌝%Z ∗
+                 ⌜s ≠ ∅⌝ ∗
+                     (* l↪ urn_unif (setprod s1  s2)∗ *)
+                     l↪ urn_unif s ∗
+                     l'↪ urn_unif s ∗
+                     ↯ (tries' / size s) ∗ ↯ (tries' / size s) ∗
+                     ⌜(S tag_range - (tries - tries')) <= size s⌝ ∗
+                   ((
+                     b ↪ urn_unif (list_to_set (Z.of_nat <$> seq 0 2)) ∗
+                     ↯ (1/2)
+                    ) ∨ ((token γ) ∗ ∃ (b_resolved : nat), ⌜b_resolved <= 1⌝ ∗ b ↪ urn_unif {[Z.of_nat b_resolved]}) )
+               )%I).
+      iMod (inv_alloc (nroot) _ inv with "[-Htoken HΦ]") as "#Hinv".
+      {
+        iNext. iExists _,_,_,_. iFrame "Hr".
+        instantiate (1 := ∅). rewrite kmap_empty. iFrame "Hf".
+        iSplit => //.
+        iFrame.
+        (* NoDup_fmap NoDup_seq *)
+        admit.
+      }
+
+    wp_bind (v _)%E.
+    rewrite refines_eq /refines_def.
+    simpl.
+    iApply (pgl_wp_wand); first iApply "Hinterp".
+    { admit. }
+    iIntros "%v' #Hv'".
+    wp_bind (v' _)%E.
+    rewrite refines_eq /refines_def.
+    iApply (pgl_wp_wand); first iApply "Hv'".
+    { admit. }
+    iIntros "%v'' #Hv''".
+    wp_bind (v'' _)%E.
+    rewrite refines_eq /refines_def.
+    iApply (pgl_wp_wand); first iApply "Hv''".
+    (* this is the actual interesting bit *)
+    {
+      iClear "H Hinterp Hv' Hv''".
+      iModIntro.
+      iIntros (?) "[%guess ->]".
+      rewrite refines_eq/refines_def.
+      wp_pures.
+      iInv "Hinv" as ">(%tries'&%m&%x&%y&Hf&Hlt&%Htries& (%s'&%Hdisjoint1&%Hdisjoint2&%Hrange&%Hnonempty&Hurn&Hurn'&Herr&Herr'&%tries_range&Hor))" "Hclose".
+      wp_load.
+      wp_pures.
+      case_bool_decide.
+      - wp_pures.
+        iMod ("Hclose" with "[-]"); first by iFrame.
+        iModIntro.
+        iExists _. iLeft. by iSplit.
+      - wp_pures.
+        wp_load.
+        wp_pures.
+        wp_store.
+        iDestruct "Hor" as "[[Hb Herr'']|Hor]".
+        + destruct (decide (guess ∈ (( (dom m)):gset _))) as [Hlookup|].
+          { (** it has been queried before *)
+            rewrite elem_of_dom in Hlookup.
+            destruct Hlookup.
+
+            wp_apply (wp_hashfun_prev _ _ _ _ _ _ guess (l↪ _) with "[$Hurn $Hf]").
+            - done.
+            -
+          }
+
+
+
+      admit. }
+
+    iIntros "% (%guess & ->)". wp_pure. wp_pure.
+    rewrite -(fill_empty (_=_)).
+    iApply (pgl_wp_bind).
+    wp_pures. simpl.
+    iInv "Hinv" as ">(%&%&%&%&?&?&?&%&?&?&?&?&?&?&?&?&?&[[b err] | (Htoken' & ?) ])" "Hclose" ; last first.
+    1: iDestruct (token_exclusive with "[$][$]") as "[]".
+    iMod (pupd_resolve_urn _ _ (λ x, if bool_decide (x=guess) then nnreal_one else nnreal_zero) with "[$err][$b]") as "(%&?&Hurn&%)".
+    1: admit.
+    (* + erewrite (SeriesC_ext _ (λ x, if bool_decide (x=guess) then nnreal_one else nnreal_zero)); last first.
+         * intros. simpl.
+           case_bool_decide as K1; first by case_bool_decide.
+           rewrite bool_decide_eq_false_2; first done.
+           intros ->. apply K1. set_solver.
+         * rewrite SeriesC_singleton.
+           simpl.
+           rewrite !Rdiv_def.
+           apply Rmult_le_compat_r.
+           -- rewrite -Rdiv_1_l.
+              apply Rdiv_INR_ge_0.
+           -- replace 1%R with (INR 1) by done.
+              apply le_INR.
+              lia. *)
+    1: admit.
+    1: exists 1 ; intros ; case_bool_decide ; simpl ; try lra.
+    case_bool_decide ; first by iDestruct (ec_contradict with "[$]") as "[]".
+        iApply (wp_value_promotion _ false (b↪ _) with "[Hurn]").
+        * rewrite rupd_unseal/rupd_def.
+          iIntros  (?) "[? Hu]". iSplit; last iFrame.
+          iDestruct (ghost_map_lookup with "Hu [$]") as "%Hlookup".
+          iPureIntro.
+          intros.
+          eapply urns_f_distr_lookup in Hlookup; last done; last done.
+          destruct Hlookup as (?&Hsome&Hin).
+          simpl.
+          rewrite Hsome.
+          simpl.
+          rewrite bool_decide_eq_false_2; first naive_solver.
+          set_unfold.
+          destruct!/=. intros ?. simplify_eq.
+        * iIntros "Hurn".
+          wp_pures.
+          iMod ("Hclose" with "[-HΦ]").
+          { iNext.
+            iFrame.
+            iRight. iFrame.
+            iExists (Z.to_nat x0). repeat iSplit; try done.
+            - iPureIntro.
+              admit.
+            - admit.
+          }
+          by iApply "HΦ".
+
+
+  Qed.
+
+
+  (*   { iModIntro. *)
+  (*     iIntros (?) "[%guess ->]". *)
+  (*     rewrite refines_eq/refines_def. *)
+  (*     wp_pures. *)
+  (*     iInv "Hinv" as ">(%tries'&%m&Hf&Hl&%& (%s'&%Hdisjoint&%Hnonempty&Hurn &Hor))" "Hclose". *)
+  (*     wp_load. *)
+  (*     wp_pures. *)
+  (*     case_bool_decide. *)
+  (*     - wp_pures. *)
+  (*       iMod ("Hclose" with "[-]"); first by iFrame. *)
+  (*       iModIntro. *)
+  (*       iExists _. iLeft. by iSplit. *)
+  (*     - wp_pures. *)
+  (*       wp_load.  *)
+  (*       wp_pures. *)
+  (*       wp_store. *)
+  (*       iDestruct "Hor" as "[Hor|Hor]". *)
+  (*       + (** normal case *) *)
+  (*         destruct (decide (guess ∈ (( (dom m)):gset _))) as [Hlookup|]. *)
+  (*         { (** it has been queried before *) *)
+  (*           rewrite elem_of_dom in Hlookup. *)
+  (*           destruct Hlookup. *)
+
+  (*           wp_apply (wp_hashfun_prev _ _ _ _ _ _ guess (l↪ _) with "[$Hurn $Hf]"). *)
+  (*           - done. *)
+  (*           - simplify_map_eq. *)
+  (*             erewrite lookup_kmap_Some; first naive_solver. *)
+  (*             intros ???. by simplify_eq. *)
+  (*           - iSplit. *)
+  (*             + iModIntro. *)
+  (*               iIntros. *)
+  (*               rewrite rupd_unseal/rupd_def. *)
+  (*               iIntros  (?) "[? Hu]". iSplit; last iFrame. *)
+  (*               iDestruct (ghost_map_lookup with "Hu [$]") as "%Hlookup". *)
+  (*               iPureIntro. *)
+  (*               intros. simpl. case_bool_decide; naive_solver. *)
+  (*             + iModIntro. *)
+  (*               iApply big_sepS_intro. *)
+  (*               iModIntro. *)
+  (*               setoid_rewrite elem_of_difference. *)
+  (*               iIntros (?) "[%Hlookup' %]". *)
+  (*               iIntros "?". *)
+  (*               rewrite rupd_unseal/rupd_def. *)
+  (*               iIntros  (?) "[? Hu]". iSplit; last iFrame. *)
+  (*               iDestruct (ghost_map_lookup with "Hu [$]") as "%Hlookup". *)
+  (*               iPureIntro. *)
+  (*               intros. *)
+  (*               eapply urns_f_distr_lookup in Hlookup; last done; last done. *)
+  (*               destruct Hlookup as (?&Hsome&Hin). *)
+  (*               eexists _; split; last done. *)
+  (*               simpl. *)
+  (*               rewrite elem_of_dom in Hlookup'. *)
+  (*               destruct Hlookup' as [? Hlookup']. *)
+  (*               rewrite lookup_insert_Some in Hlookup'. *)
+  (*               destruct!/=. *)
+  (*               * rewrite Hsome/=. rewrite bool_decide_eq_false_2; first done. *)
+  (*                 intros ?. simplify_eq. *)
+  (*                 apply Hdisjoint in Hin. *)
+  (*                 apply Hin. *)
+  (*                 rewrite elem_of_dom. naive_solver. *)
+  (*               * rename select (kmap _ _ !! _ = _) into K1. *)
+  (*                 apply lookup_kmap_Some in K1; last (intros ???; by simplify_eq). *)
+  (*                 destruct!/=. rewrite bool_decide_eq_false_2; first done. *)
+  (*                 intros ?. simplify_eq. *)
+  (*                 set_unfold. simplify_eq. *)
+  (*           - iIntros "[Hf Hu]". *)
+  (*             wp_pures. *)
+  (*             iMod ("Hclose" with "[Hl Hf Hu Hor]"). *)
+  (*             { iNext. *)
+  (*               iFrame "Hf Hu". *)
+  (*               replace (Z.of_nat _ -_)%Z with (Z.of_nat (tries' - 1)); last first.  *)
+  (*               { assert (tries' ≠ 0)%nat; last lia. *)
+  (*                 by intros ->. *)
+  (*               } *)
+  (*               iFrame "Hl". *)
+  (*               repeat iSplit. *)
+  (*               - iPureIntro; lia. *)
+  (*               - done. *)
+  (*               - done. *)
+  (*               - iLeft. *)
+  (*                 iDestruct "Hor" as "(%&Herr&Herr'&%)". *)
+  (*                 repeat iSplit. *)
+  (*                 + done. *)
+  (*                 + iSplitL "Herr"; last repeat iSplit. *)
+  (*                   * iApply (ec_weaken with "[$]"). *)
+  (*                     replace 1%R with (INR 1) by done. *)
+  (*                     rewrite -!plus_INR. *)
+  (*                     split; first apply INR_div_pos. *)
+  (*                     rewrite !Rdiv_def. *)
+  (*                     apply Rmult_le_compat_r. *)
+  (*                     -- rewrite -Rdiv_1_l. *)
+  (*                        apply Rdiv_INR_ge_0. *)
+  (*                     -- apply le_INR. lia. *)
+  (*                   * iApply (ec_weaken with "[$]"). *)
+  (*                     split; first apply INR_div_pos. *)
+  (*                     rewrite !Rdiv_def. *)
+  (*                     apply Rmult_le_compat_r. *)
+  (*                     -- rewrite -Rdiv_1_l. *)
+  (*                        apply Rdiv_INR_ge_0. *)
+  (*                     -- apply le_INR. lia. *)
+  (*                   * iPureIntro. lia. *)
+  (*             } *)
+  (*             iModIntro. *)
+  (*             iExists _. iRight. *)
+  (*             iSplit; first done. *)
+  (*             by iExists _. *)
+  (*         } *)
+  (*         (** Not queries before *) *)
+  (*         iDestruct "Hor" as "(%&Herr1&Herr2&%)". *)
+  (*         assert (tries' ≠ 0). *)
+  (*         { intros ?. simplify_eq. } *)
+  (*         iAssert (pupd ∅ ∅ (∃s'', ⌜ s'' ⊆ s' ⌝ ∗ ⌜ s''≠∅⌝ ∗ *)
+  (*                                  l ↪ urn_unif s'' ∗ ⌜guess∉ s''⌝ ∗ *)
+  (*                                  ⌜size s'<=size s''+1⌝ ∗ *)
+  (*                                  ↯ ((tries'-1+1)%nat/size s'') *)
+  (*                 ))%I with "[Hurn Herr2]" as ">H'". *)
+  (*         { destruct (decide (guess ∈ s')); last first. *)
+  (*          - iModIntro. *)
+  (*            iFrame. *)
+  (*            repeat iSplit; try done. *)
+  (*            + iPureIntro; lia. *)
+  (*            + iApply (ec_weaken with "[$]"). *)
+  (*              split. *)
+  (*              * apply INR_div_pos. *)
+  (*              * rewrite !Rdiv_def. *)
+  (*                apply Rmult_le_compat_r. *)
+  (*                -- rewrite -Rdiv_1_l. apply Rdiv_INR_ge_0. *)
+  (*                -- apply le_INR. lia. *)
+  (*          - assert (0<= (tries'-1+1)%nat/(size s' -1)%nat)%R as err_ineq. *)
+  (*            { apply INR_div_pos. } *)
+  (*            iAssert (⌜2<=size s'⌝)%I as "%". *)
+  (*            { destruct (size s') as [|[|]]eqn:Hcontra; last (iPureIntro; lia). *)
+  (*              - apply size_empty_inv in Hcontra. *)
+  (*                by rewrite leibniz_equiv_iff in Hcontra. *)
+  (*              - iDestruct (ec_contradict with "[$]") as "[]". *)
+  (*                simpl. *)
+  (*                rewrite Rdiv_1_r. *)
+  (*                replace 1%R with (INR 1) by done. *)
+  (*                apply le_INR. lia. *)
+  (*            } *)
+  (*            iMod (pupd_partial_resolve_urn _ _ (λ x, if bool_decide (x=({[guess]} : gset _)) then nnreal_one else mknonnegreal _ err_ineq) _ _ (({[guess]} ::(s'∖{[guess]}) ::[]): list (gset _)) with "[$][$]") as "H'". *)
+  (*            + done. *)
+  (*            + simpl. *)
+  (*              rewrite union_empty_r_L. *)
+  (*              rewrite -union_difference_L; first done. *)
+  (*              set_solver. *)
+  (*            + repeat setoid_rewrite NoDup_cons. *)
+  (*              repeat split; last by apply NoDup_nil. *)
+  (*              -- set_unfold. *)
+  (*                 intros ?. destruct!/=. set_solver. *)
+  (*              -- set_solver. *)
+  (*            + set_unfold. *)
+  (*              intros ?. *)
+  (*              destruct!/=. *)
+  (*              rename select (_=_∖_) into Hcontra. *)
+  (*              apply (f_equal size) in Hcontra. *)
+  (*              rewrite size_empty size_difference in Hcontra; last set_solver. *)
+  (*              rewrite size_singleton in Hcontra. lia. *)
+  (*            + intros. *)
+  (*              set_unfold. *)
+  (*              destruct!/=; set_solver. *)
+  (*            + rewrite SeriesC_list; last first. *)
+  (*              { repeat setoid_rewrite NoDup_cons. *)
+  (*                repeat split; last by apply NoDup_nil. *)
+  (*                - set_unfold. *)
+  (*                  intros ?. destruct!/=. set_solver. *)
+  (*                - set_solver. } *)
+  (*              Local Opaque size. *)
+  (*              simpl. *)
+  (*              rewrite bool_decide_eq_true_2; last done. *)
+  (*              rewrite Rmult_1_l size_singleton. *)
+  (*              rewrite bool_decide_eq_false_2; last set_solver. *)
+  (*              rewrite Rplus_0_r. *)
+  (*              simpl. *)
+  (*              rewrite size_difference; last set_solver. *)
+
+  (*              replace (_-_+_) with tries' by lia. *)
+  (*              rewrite !Rdiv_def. *)
+  (*              apply Rmult_le_compat_r. *)
+  (*              * rewrite -Rdiv_1_l. *)
+  (*                apply Rdiv_INR_ge_0. *)
+  (*              * rewrite size_singleton. *)
+  (*                rewrite plus_INR. *)
+  (*                simpl. *)
+  (*                rewrite Rmult_assoc. *)
+  (*                rewrite (Rmult_comm (/ _)%R). *)
+  (*                assert ((size s' - 1)%nat */(size s' -1)%nat=1)%R as ->; last lra. *)
+  (*                rewrite -Rdiv_def. *)
+  (*                rewrite Rdiv_diag; first done. *)
+  (*                rewrite minus_INR; last lia. *)
+  (*                simpl. *)
+  (*                assert (INR (size s') ≠ 1)%R; last lra. *)
+  (*                replace 1%R with (INR 1) by done. *)
+  (*                apply not_INR. lia.  *)
+  (*            + eexists (Rmax _ _). *)
+  (*              intros. *)
+  (*              case_bool_decide. *)
+  (*              -- apply Rmax_l. *)
+  (*              -- apply Rmax_r. *)
+  (*            + iDestruct "H'" as "(%&Herr&Hurn &%)". *)
+  (*              set_unfold. *)
+  (*              destruct!/=. *)
+  (*              * rewrite bool_decide_eq_true_2; last done. *)
+  (*                by iDestruct (ec_contradict with "[$]") as "[]". *)
+  (*              * rewrite bool_decide_eq_false_2; last set_solver. *)
+  (*                iFrame. *)
+  (*                iModIntro. *)
+  (*                repeat iSplit; try iPureIntro. *)
+  (*                -- set_solver. *)
+  (*                -- intros Hcontra. *)
+  (*                   apply (f_equal size) in Hcontra. *)
+  (*                   rewrite size_empty size_difference in Hcontra; last set_solver. *)
+  (*                   rewrite size_singleton in Hcontra. lia. *)
+  (*                -- set_solver. *)
+  (*                -- rewrite size_difference; last set_solver. *)
+  (*                   rewrite size_singleton. lia. *)
+  (*                -- iApply (ec_eq with "[$]"). *)
+  (*                   simpl. rewrite size_difference; last set_solver. *)
+  (*                   by rewrite size_singleton. *)
+  (*         } *)
+  (*         iDestruct "H'" as "(%s''&%&%&Hurn&%Hnotin&%Hsize'&Herr2)". *)
+  (*         replace (_/_)%R with (((tries'-1)%nat+1)/(val_size+1)%nat+1/(val_size+1)%nat)%R; last first. *)
+  (*         { rewrite -Rdiv_plus_distr. f_equal. f_equal. *)
+  (*           rewrite minus_INR; last lia. *)
+  (*           simpl. *)
+  (*           lra.  *)
+  (*         } *)
+  (*         iDestruct (ec_split with "[$]") as "[Herr1 Herr1']". *)
+  (*         { replace 1%R with (INR 1) by done. rewrite -plus_INR. *)
+  (*           apply INR_div_pos. *)
+  (*         } *)
+  (*         { replace 1%R with (INR 1) by done. apply INR_div_pos. } *)
+  (*         wp_apply (wp_insert_new _ _ _ _ _ _ (λ x, if bool_decide (x= secret) then nnreal_one else nnreal_zero)%R (l↪ _) with "[$Hf $Herr1' $Hurn]"). *)
+  (*         * done. *)
+  (*         * intros. case_bool_decide; simpl; lra. *)
+  (*         * rewrite SeriesC_scal_l. *)
+  (*           rewrite SeriesC_singleton. *)
+  (*           rewrite Rmult_1_r. *)
+  (*           rewrite S_INR. *)
+  (*           by rewrite plus_INR. *)
+  (*         * iModIntro. *)
+  (*           iApply big_sepS_intro. *)
+  (*           iModIntro. *)
+  (*           iIntros (?) "%Hlookup'". *)
+  (*           iIntros "?". *)
+  (*           rewrite rupd_unseal/rupd_def. *)
+  (*           iIntros  (?) "[? Hu]". iSplit; last iFrame. *)
+  (*           iDestruct (ghost_map_lookup with "Hu [$]") as "%Hlookup". *)
+  (*           iPureIntro. *)
+  (*           intros. *)
+  (*           eapply urns_f_distr_lookup in Hlookup; last done; last done. *)
+  (*           destruct Hlookup as (?&Hsome&Hin). *)
+  (*           eexists _; split; last done. *)
+  (*           simpl. *)
+  (*           rewrite elem_of_dom in Hlookup'. *)
+  (*           destruct Hlookup' as [? Hlookup']. *)
+  (*           rewrite lookup_insert_Some in Hlookup'. *)
+  (*           destruct!/=. *)
+  (*           -- rewrite Hsome/=. rewrite bool_decide_eq_false_2; first done. *)
+  (*              intros ?. simplify_eq. *)
+  (*           -- rename select (kmap _ _ !! _ = _) into K1. *)
+  (*              apply lookup_kmap_Some in K1; last (intros ???; by simplify_eq). *)
+  (*              destruct!/=. rewrite bool_decide_eq_false_2; first done. *)
+  (*              intros ?. simplify_eq. *)
+  (*              rename select (m!!_=Some _) into Hcontra. *)
+  (*              apply elem_of_dom_2 in Hcontra. *)
+  (*              set_solver. *)
+  (*         * iIntros (?) "(Hf&Hurn&Herr)". *)
+  (*           case_bool_decide. *)
+  (*           { by iDestruct (ec_contradict with "[$]") as "[]". } *)
+  (*           wp_pures. *)
+  (*           iMod ("Hclose" with "[-Herr]"). *)
+  (*           { iNext. *)
+  (*             replace (Z.of_nat _ - _)%Z with (Z.of_nat (tries'-1)) by lia. *)
+  (*             iFrame "Hl". iFrame "Hurn". *)
+  (*             iExists _. *)
+  (*             erewrite kmap_insert; last (intros ???; by simplify_eq). *)
+  (*             rewrite insert_commute; last done. *)
+  (*             iFrame. *)
+  (*             repeat iSplit; last iLeft; repeat iSplit. *)
+  (*             - iPureIntro; lia. *)
+  (*             - iPureIntro. set_unfold. set_solver. *)
+  (*             - done. *)
+  (*             - iPureIntro. *)
+  (*               intros ?? Hlookup'. *)
+  (*               apply lookup_insert_Some in Hlookup'. *)
+  (*               destruct!/=. *)
+  (*               + intros Hcontra. *)
+  (*                 by apply fin_to_nat_inj in Hcontra. *)
+  (*               + naive_solver. *)
+  (*             - rewrite (plus_INR (_-_)). iFrame. *)
+  (*               iPureIntro. lia. *)
+  (*           } *)
+  (*           iExists _. iModIntro. *)
+  (*           iRight. *)
+  (*           iSplit; first done. *)
+  (*           by iExists _. *)
+  (*       + (** token case, its a weird case *) *)
+  (*         assert (tries' ≠ 0). *)
+  (*         { intros ->. simplify_eq. } *)
+  (*         iMod (ec_zero) as "Herr". *)
+  (*         iMod (pupd_resolve_urn _ _ (λ _, nnreal_zero) with "[$][$]") as "(%&_&Hurn&%)". *)
+  (*         * done. *)
+  (*         * rewrite SeriesC_0; first lra. *)
+  (*           intros. *)
+  (*           by case_bool_decide. *)
+  (*         * naive_solver. *)
+  (*         * destruct (decide (guess ∈ dom m)) as [Hlookup|]. *)
+  (*           (** queried before *) *)
+  (*           { rewrite elem_of_dom in Hlookup. *)
+  (*             destruct Hlookup. *)
+  (*             wp_apply (wp_hashfun_prev _ _ _ _ _ _ guess (l↪ _) with "[$Hurn $Hf]"). *)
+  (*             - done. *)
+  (*             - rewrite lookup_insert_Some. right. split; first done. *)
+  (*               erewrite lookup_kmap_Some; last (intros ???; by simplify_eq). *)
+  (*               naive_solver. *)
+  (*             - iSplit. *)
+  (*               + iModIntro. *)
+  (*                 iIntros. *)
+  (*                 rewrite rupd_unseal/rupd_def. *)
+  (*                 iIntros  (?) "[? Hu]". iSplit; last iFrame. *)
+  (*                 iDestruct (ghost_map_lookup with "Hu [$]") as "%Hlookup". *)
+  (*                 iPureIntro. *)
+  (*                 intros. simpl. case_bool_decide; naive_solver. *)
+  (*               + iModIntro. *)
+  (*                 iApply big_sepS_intro. *)
+  (*                 iModIntro. *)
+  (*                 setoid_rewrite elem_of_difference. *)
+  (*                 iIntros (?) "[%Hlookup' %]". *)
+  (*                 iIntros "?". *)
+  (*                 rewrite rupd_unseal/rupd_def. *)
+  (*                 iIntros  (?) "[? Hu]". iSplit; last iFrame. *)
+  (*                 iDestruct (ghost_map_lookup with "Hu [$]") as "%Hlookup". *)
+  (*                 iPureIntro. *)
+  (*                 intros. *)
+  (*                 eapply urns_f_distr_lookup in Hlookup; last done; last done. *)
+  (*                 destruct Hlookup as (?&Hsome&Hin). *)
+  (*                 eexists _; split; last done. *)
+  (*                 simpl. *)
+  (*                 rewrite elem_of_dom in Hlookup'. *)
+  (*                 destruct Hlookup' as [? Hlookup']. *)
+  (*                 rewrite lookup_insert_Some in Hlookup'. *)
+  (*                 destruct!/=. *)
+  (*                 * rewrite Hsome/=. rewrite bool_decide_eq_false_2; first done. *)
+  (*                   intros ?. simplify_eq. *)
+  (*                   set_unfold. destruct!/=. *)
+  (*                   eapply Hdisjoint; first done. *)
+  (*                   setoid_rewrite elem_of_dom. naive_solver. *)
+  (*                 * rename select (kmap _ _ !! _ = _) into K1. *)
+  (*                   apply lookup_kmap_Some in K1; last (intros ???; by simplify_eq). *)
+  (*                   destruct!/=. rewrite bool_decide_eq_false_2; first done. *)
+  (*                   intros ?. simplify_eq. *)
+  (*                   set_unfold. simplify_eq.  *)
+  (*             - iIntros "[Hf Hurn]". *)
+  (*               wp_pures. *)
+  (*               iMod ("Hclose" with "[-]"). *)
+  (*               { iNext. *)
+  (*                 replace (Z.of_nat _ - _)%Z with (Z.of_nat (tries' - 1)) by lia. *)
+  (*                 iFrame "Hl Hf Hurn". *)
+  (*                 repeat iSplit; last iRight; last iFrame; iPureIntro.  *)
+  (*                 - lia. *)
+  (*                 - set_solver. *)
+  (*                 - done.  *)
+  (*               } *)
+  (*               iModIntro. *)
+  (*               iExists _. iRight. *)
+  (*               iSplit; first done. *)
+  (*               by iExists _. *)
+  (*           } *)
+  (*           destruct (decide (guess = x)). *)
+  (*           { (** guess is x*) *)
+  (*             wp_apply (wp_hashfun_prev _ _ _ _ _ _ (LitLbl l) (l↪ _) with "[$Hurn $Hf]"). *)
+  (*             - done. *)
+  (*             - rewrite lookup_insert_Some. naive_solver. *)
+  (*             - iSplit. *)
+  (*               + iModIntro. *)
+  (*                 iIntros. *)
+  (*                 rewrite rupd_unseal/rupd_def. *)
+  (*                 iIntros  (?) "[? Hu]". iSplit; last iFrame. *)
+  (*                 iDestruct (ghost_map_lookup with "Hu [$]") as "%Hlookup". *)
+  (*                 iPureIntro. *)
+  (*                 intros. simpl. *)
+  (*                 eapply urns_f_distr_lookup in Hlookup; last done; last done. *)
+  (*                 destruct Hlookup as (?&Hsome&Hin). *)
+  (*                 eexists _; split; last done. *)
+  (*                 rewrite Hsome. simpl. *)
+  (*                 set_unfold. destruct!/=. *)
+  (*                 by case_bool_decide.  *)
+  (*               + iModIntro. *)
+  (*                 iApply big_sepS_intro. *)
+  (*                 iModIntro. *)
+  (*                 setoid_rewrite elem_of_difference. *)
+  (*                 iIntros (?) "[%Hlookup' %]". *)
+  (*                 iIntros "?". *)
+  (*                 rewrite rupd_unseal/rupd_def. *)
+  (*                 iIntros  (?) "[? Hu]". iSplit; last iFrame. *)
+  (*                 iDestruct (ghost_map_lookup with "Hu [$]") as "%Hlookup". *)
+  (*                 iPureIntro. *)
+  (*                 intros. *)
+  (*                 eapply urns_f_distr_lookup in Hlookup; last done; last done. *)
+  (*                 destruct Hlookup as (?&Hsome&Hin). *)
+  (*                 eexists _; split; last done. *)
+  (*                 simpl. *)
+  (*                 rewrite elem_of_dom in Hlookup'. *)
+  (*                 destruct Hlookup' as [? Hlookup']. *)
+  (*                 rewrite lookup_insert_Some in Hlookup'. *)
+  (*                 destruct!/=. *)
+  (*                 * rewrite Hsome/=. rewrite bool_decide_eq_false_2; first done. *)
+  (*                   intros ?. simplify_eq. *)
+  (*                   set_unfold. destruct!/=. *)
+  (*                 * rename select (kmap _ _ !! _ = _) into K1. *)
+  (*                   apply lookup_kmap_Some in K1; last (intros ???; by simplify_eq). *)
+  (*                   destruct!/=. rewrite bool_decide_eq_false_2; first done. *)
+  (*                   intros ?. simplify_eq. *)
+  (*                   set_unfold. simplify_eq.  *)
+  (*                   eapply Hdisjoint; first done. *)
+  (*                   setoid_rewrite elem_of_dom. naive_solver. *)
+  (*             - iIntros "[Hf Hurn]". *)
+  (*               wp_pures. *)
+  (*               iMod ("Hclose" with "[-]"). *)
+  (*               { iNext. *)
+  (*                 replace (Z.of_nat _ - _)%Z with (Z.of_nat (tries' - 1)) by lia. *)
+  (*                 iFrame "Hl Hf Hurn". *)
+  (*                 repeat iSplit; last iRight; last iFrame; iPureIntro.  *)
+  (*                 - lia. *)
+  (*                 - set_solver. *)
+  (*                 - done.  *)
+  (*               } *)
+  (*               iModIntro. *)
+  (*               iExists _. iRight. *)
+  (*               iSplit; first done. *)
+  (*               by iExists _. *)
+  (*             } *)
+  (*             (** guess is not queried before *) *)
+  (*             iMod (ec_zero) as "Herr". *)
+  (*           wp_apply (wp_insert_new _ _ _ _ _ _ (λ x, nnreal_zero)%R (l↪ _) with "[$Hf $Herr $Hurn]"). *)
+  (*           -- done. *)
+  (*           -- naive_solver. *)
+  (*           -- rewrite SeriesC_0; first done. *)
+  (*              intros. simpl. lra. *)
+  (*           -- iModIntro. *)
+  (*              iApply big_sepS_intro. *)
+  (*              iModIntro. *)
+  (*              iIntros (?) "%Hlookup'". *)
+  (*              iIntros "?". *)
+  (*              rewrite rupd_unseal/rupd_def. *)
+  (*              iIntros  (?) "[? Hu]". iSplit; last iFrame. *)
+  (*              iDestruct (ghost_map_lookup with "Hu [$]") as "%Hlookup". *)
+  (*              iPureIntro. *)
+  (*              intros. *)
+  (*              eapply urns_f_distr_lookup in Hlookup; last done; last done. *)
+  (*              destruct Hlookup as (?&Hsome&Hin). *)
+  (*              eexists _; split; last done. *)
+  (*              simpl. *)
+  (*              rewrite elem_of_dom in Hlookup'. *)
+  (*              destruct Hlookup' as [? Hlookup']. *)
+  (*              rewrite lookup_insert_Some in Hlookup'. *)
+  (*              destruct!/=. *)
+  (*              ++ rewrite Hsome/=. rewrite bool_decide_eq_false_2; first done. *)
+  (*                 intros ?. simplify_eq. *)
+  (*                 set_unfold. destruct!/=. *)
+  (*              ++ rename select (kmap _ _ !! _ = _) into K1. *)
+  (*                 apply lookup_kmap_Some in K1; last (intros ???; by simplify_eq). *)
+  (*                 destruct!/=. rewrite bool_decide_eq_false_2; first done. *)
+  (*                 set_unfold. simplify_eq. *)
+  (*                 rename select (_∉dom _) into Hcontra. *)
+  (*                 rewrite elem_of_dom in Hcontra. *)
+  (*                 intros ?. simplify_eq. naive_solver. *)
+  (*           -- iIntros (?) "(Hf&Hurn&_)". *)
+  (*              wp_pures. *)
+  (*              iMod ("Hclose" with "[-]"). *)
+  (*              { iNext. *)
+  (*                replace (Z.of_nat _ - _)%Z with (Z.of_nat (tries' - 1)) by lia. *)
+  (*                iExists _, _. *)
+  (*                erewrite kmap_insert; last (intros ???; by simplify_eq). *)
+  (*                rewrite insert_commute; last done.  *)
+  (*                iFrame "Hl Hurn Hf". *)
+  (*                repeat iSplit; last iRight; last iFrame; iPureIntro.  *)
+  (*                - lia. *)
+  (*                - set_solver. *)
+  (*                - done.  *)
+  (*              } *)
+  (*              iModIntro. *)
+  (*              iExists _. iRight. *)
+  (*              iSplit; first done. *)
+  (*              by iExists _. *)
+  (*   } *)
+  (*   (** * Final bit *) *)
+  (*   iIntros (f') "#Hinterp'". *)
+  (*   wp_bind (f' _)%E. *)
+  (*   rewrite refines_eq /refines_def. *)
+  (*   iApply (pgl_wp_wand); first iApply "Hinterp'". *)
+  (*   { iExists (nat_to_fin (fin_to_nat_lt _)). by rewrite fin_to_nat_to_fin. } *)
+  (*   iIntros (?) "[%guess ->]". *)
+  (*   wp_pures.  *)
+  (*   iInv "Hinv" as ">(%tries'&%m&Hf&Hl&%& (%s'&%Hdisjoint&%Hnonempty&Hurn &Hor))" "Hclose". *)
+  (*   iDestruct ("Hor") as "[Hor|Htoken']"; last first. *)
+  (*   { iCombine "Htoken" "Htoken'" gives "[]". } *)
+  (*   iDestruct "Hor" as "(%Hnotin&Herr&Herr'&%H1)". *)
+  (*   assert (is_valid_urn (urn_unif s')). *)
+  (*   { simpl. *)
+  (*     intros ->. *)
+  (*     rewrite size_empty in H1. lia. *)
+  (*   } *)
+
+
+  (*   destruct (decide (guess ∈ dom m)) as [Hlookup|]. *)
+  (*     -- (** Return something hashed before *) *)
+  (*       rewrite elem_of_dom in Hlookup. *)
+  (*       destruct Hlookup. *)
+
+  (*       wp_apply (wp_hashfun_prev _ _ _ _ _ _ guess (l↪ _) with "[$Hurn $Hf]"). *)
+  (*       ++ done. *)
+  (*       ++ simplify_map_eq. *)
+  (*          erewrite lookup_kmap_Some; first naive_solver. *)
+  (*          intros ???. by simplify_eq. *)
+  (*       ++ iSplit. *)
+  (*          ** iModIntro. *)
+  (*             iIntros. *)
+  (*             rewrite rupd_unseal/rupd_def. *)
+  (*             iIntros  (?) "[? Hu]". iSplit; last iFrame. *)
+  (*             iDestruct (ghost_map_lookup with "Hu [$]") as "%Hlookup". *)
+  (*             iPureIntro. *)
+  (*             intros. simpl. case_bool_decide; naive_solver. *)
+  (*          ** iModIntro. *)
+  (*             iApply big_sepS_intro. *)
+  (*             iModIntro. *)
+  (*             setoid_rewrite elem_of_difference. *)
+  (*             iIntros (?) "[%Hlookup' %]". *)
+  (*             iIntros "?". *)
+  (*             rewrite rupd_unseal/rupd_def. *)
+  (*             iIntros  (?) "[? Hu]". iSplit; last iFrame. *)
+  (*             iDestruct (ghost_map_lookup with "Hu [$]") as "%Hlookup". *)
+  (*             iPureIntro. *)
+  (*             intros. *)
+  (*             eapply urns_f_distr_lookup in Hlookup; last done; last done. *)
+  (*             destruct Hlookup as (?&Hsome&Hin). *)
+  (*             eexists _; split; last done. *)
+  (*             simpl. *)
+  (*             rewrite elem_of_dom in Hlookup'. *)
+  (*             destruct Hlookup' as [? Hlookup']. *)
+  (*             rewrite lookup_insert_Some in Hlookup'. *)
+  (*             destruct!/=. *)
+  (*             --- rewrite Hsome/=. rewrite bool_decide_eq_false_2; first done. *)
+  (*                 intros ?. simplify_eq. *)
+  (*                 apply Hdisjoint in Hin. *)
+  (*                 apply Hin. *)
+  (*                 rewrite elem_of_dom. naive_solver. *)
+  (*             --- rename select (kmap _ _ !! _ = _) into K1. *)
+  (*                 apply lookup_kmap_Some in K1; last (intros ???; by simplify_eq). *)
+  (*                 destruct!/=. rewrite bool_decide_eq_false_2; first done. *)
+  (*                 intros ?. simplify_eq. *)
+  (*                 set_unfold. simplify_eq. *)
+  (*       ++ iIntros "[Hf Hu]". *)
+  (*          wp_pures. *)
+  (*          rewrite bool_decide_eq_false_2; last first. *)
+  (*          { intros ?. simplify_eq. *)
+  (*            naive_solver. *)
+  (*          } *)
+  (*          iMod ("Hclose" with "[Htoken Hl Hf Hu]"). *)
+  (*          { iNext. *)
+  (*            iFrame "Hl Hf Hu". *)
+  (*            repeat iSplit; try done. *)
+  (*            by iRight.  *)
+  (*          } *)
+  (*          by iApply "HΦ". *)
+  (*     -- iAssert (pupd ∅ ∅ (∃s'', ⌜ s'' ⊆ s' ⌝ ∗ ⌜ s''≠∅⌝ ∗ *)
+  (*                                 l ↪ urn_unif s'' ∗ ⌜guess∉ s''⌝ *)
+  (*                ))%I with "[Herr' Hurn]" as ">H'". *)
+  (*        { destruct (decide (guess ∈ s')); last first. *)
+  (*          - iModIntro. *)
+  (*            iFrame. *)
+  (*            iPureIntro. simpl in *. naive_solver. *)
+  (*          - iMod (pupd_resolve_urn _ _ (λ x, if bool_decide (x=guess) then nnreal_one else nnreal_zero) with "[$][$]") as "(%&?&?&%)". *)
+  (*            + done. *)
+  (*            + erewrite (SeriesC_ext _ (λ x, if bool_decide (x=guess) then nnreal_one else nnreal_zero)); last first. *)
+  (*              -- intros. *)
+  (*                 case_bool_decide as H3; first by case_bool_decide. *)
+  (*                 rewrite bool_decide_eq_false_2; first done. *)
+  (*                 intros ->. apply H3. set_solver. *)
+  (*              -- rewrite SeriesC_singleton. *)
+  (*                 simpl. *)
+  (*                 rewrite !Rdiv_def. *)
+  (*                 apply Rmult_le_compat_r. *)
+  (*                 ++ rewrite -Rdiv_1_l. *)
+  (*                    apply Rdiv_INR_ge_0. *)
+  (*                 ++ replace 1%R with (INR 1) by done. *)
+  (*                    apply le_INR. *)
+  (*                    lia. *)
+  (*            + exists 1. *)
+  (*              intros. *)
+  (*              case_bool_decide; simpl; lra. *)
+  (*            + case_bool_decide. *)
+  (*              * by iDestruct (ec_contradict with "[$]") as "[]". *)
+  (*              * iFrame. *)
+  (*                iModIntro. *)
+  (*                iPureIntro. *)
+  (*                set_solver.        *)
+  (*        } *)
+  (*        iDestruct "H'" as "(%s''&%&%&Hurn &%)". *)
+  (*        wp_apply (wp_insert_new _ _ _ _ _ _ (λ x, if bool_decide (x= secret) then nnreal_one else nnreal_zero)%R (l↪ _) with "[$Hf $Herr $Hurn]"). *)
+  (*        ++ done. *)
+  (*        ++ intros. case_bool_decide; simpl; lra. *)
+  (*        ++ rewrite SeriesC_scal_l. rewrite SeriesC_singleton. *)
+  (*           rewrite Rmult_1_r. *)
+  (*           rewrite S_INR. *)
+  (*           replace 1%R with (INR 1) by done. *)
+  (*           rewrite -!plus_INR. *)
+  (*           simpl. *)
+  (*           rewrite !Rdiv_def. *)
+  (*           apply Rmult_le_compat_r. *)
+  (*           ** rewrite -Rdiv_1_l. *)
+  (*              apply Rdiv_INR_ge_0. *)
+  (*           ** replace 1%R with (INR 1) by done. *)
+  (*              apply le_INR. *)
+  (*              lia. *)
+  (*        ++ iModIntro. *)
+  (*           iApply big_sepS_intro. *)
+  (*           iModIntro. *)
+  (*           iIntros (?) "%Hlookup'". *)
+  (*           iIntros "?". *)
+  (*           rewrite rupd_unseal/rupd_def. *)
+  (*           iIntros  (?) "[? Hu]". iSplit; last iFrame. *)
+  (*           iDestruct (ghost_map_lookup with "Hu [$]") as "%Hlookup". *)
+  (*           iPureIntro. *)
+  (*           intros. *)
+  (*           eapply urns_f_distr_lookup in Hlookup; last done; last done. *)
+  (*           destruct Hlookup as (?&Hsome&Hin). *)
+  (*           eexists _; split; last done. *)
+  (*           simpl. *)
+  (*           rewrite elem_of_dom in Hlookup'. *)
+  (*           destruct Hlookup' as [? Hlookup']. *)
+  (*           rewrite lookup_insert_Some in Hlookup'. *)
+  (*           destruct!/=. *)
+  (*           ** rewrite Hsome/=. *)
+  (*              rewrite bool_decide_eq_false_2; first done. *)
+  (*              intros ?. simplify_eq. *)
+  (*           ** rename select (kmap _ _ !!_=_) into Hlookup'. *)
+  (*              apply lookup_kmap_Some in Hlookup'; last (intros ???; by simplify_eq). *)
+  (*              destruct!/=. *)
+  (*              rewrite bool_decide_eq_false_2; first done. *)
+  (*              intros ?. simplify_eq. *)
+  (*              rename select (m!!_=Some _) into Hcontra. *)
+  (*              apply elem_of_dom_2 in Hcontra. *)
+  (*              set_solver. *)
+  (*        ++ iIntros (?) "(Hf&Hurn &Herr)". *)
+  (*           case_bool_decide. *)
+  (*           { by iDestruct (ec_contradict with "[$]") as "[]". } *)
+  (*           wp_pures. *)
+  (*           iMod ("Hclose" with "[-HΦ]"). *)
+  (*           { iNext. *)
+  (*             iFrame "Hl". *)
+  (*             rewrite insert_commute; last done. *)
+  (*             iExists _. *)
+  (*             erewrite kmap_insert; first iFrame "Hf"; last (intros ???; by simplify_eq). *)
+  (*             iSplit; first done. *)
+  (*             iFrame "Hurn". *)
+  (*             repeat iSplit; last by iRight. *)
+  (*             - iPureIntro. *)
+  (*               set_solver. *)
+  (*             - done. *)
+  (*           } *)
+  (*           iApply "HΦ". *)
+  (*           iModIntro. *)
+  (*           iPureIntro. *)
+  (*           split; first done. *)
+  (*           rewrite bool_decide_eq_false_2; first done. *)
+  (*           intros ?. simplify_eq. *)
+  (* Qed. *)
+
+
+(* attempt at the proof for a single product-urn *)
   Lemma basic_hash_game A:
     ∅ ⊢ₜ A : ((TInt* TInt) → (TInt* TInt) → (TInt → (TUnit+TInt))  → TInt) ->
              pgl (lim_exec ((prog A), {|heap:=∅; urns:= ∅|})) (λ v, v=#false)
@@ -250,8 +1339,14 @@ Section prog.
 
      Hence the error is 2*(tries)/(S tag_range) + 1/2
    *)
-      assert (gset Z -> gset Z -> gset Z ) as setprod.
-      1: admit.
+      set (ff (x y : Z) := (x * tag_range + y)%Z).
+      set (f' := (λ (xy : Z * Z), ff xy.1 xy.2)).
+      set (g (s1 s2 : gset Z) := (cprod s1 s2 : gset (Z * Z))).
+      set (h := set_map (A := (Z*Z)) (B := Z)
+                  (C := gset (Z*Z))
+                  (D := gset Z)
+                   f').
+      set (setprod (s1 s2 : gset Z) := h (g s1 s2)).
       set (n1_b_n2_T2 := ((n2 * (tag_range + 1))%Z +ᵥ
                ((LitLbl b *ᵥ QuotOp' (LitLbl l) (tag_range + 1)%Z) +ᵥ
                 ((1%Z -ᵥ LitLbl b) *ᵥ RemOp' (LitLbl l) (tag_range + 1)%Z)))%V).
@@ -286,7 +1381,10 @@ Section prog.
       {
         iNext. iExists _,_,_,_. iFrame "Hr".
         instantiate (1 := ∅). rewrite kmap_empty. iFrame "Hf".
-        iSplit => //. iExists _,_.
+        iSplit => //.
+        set (s := (list_to_set (Z.of_nat <$> seq 0 (S ((tag_range + 1) * (tag_range + 1) - 1))))).
+        pose ()
+        iExists _,_.
   Abort.
 
   (*     iAssert (∃s, l↪urn_unif s ∗ ⌜size s = S secret_range⌝)%I with "[$Hl]" as "H'". *)
